\def\duedate{08/31/2022}
\def\HWnum{1}
\input{../preamble.tex}

\begin{document}
    
\prob{1.2}{Derive the cyclicity (1.24) of the trace from Eq. (1.23).}

Using the definition of the trace, we can write
\begin{eqnarray}
    \label{eq:trace-AB}
    {\rm Tr}(AB) = \sum_{k=1}^{n} (AB)_{kk} = \sum_{k=1}^{n} \sum_{\ell=1}^{n} A_{k\ell}B_{\ell k}
.\end{eqnarray}
Note that this sum is symmetric in the indices $\{ k,\ell \} $, and since $A_{k\ell}$ and $B_{\ell k}$ are just scalars 
\begin{eqnarray}
    \label{eq:trace-BA}
    \eqbox{
    {\rm Tr}(AB) = \sum_{\ell=1}^{n} \sum_{k=1}^{n} B_{\ell k}A_{k\ell} = {\rm Tr}(BA)
    } 
.\end{eqnarray}


\prob{1.3}{Show that $\left( AB \right)^{\rm T} = B^{\rm T}A^{\rm T}$, which is Eq.~(1.26).}

Recall the definition of a matrix transpose: $(A^{\rm T})_{ij} = A_{ji}$, so
\begin{eqnarray}
    \label{eq:transpose-AB}
    (AB)^{\rm T}_{ij} = (AB)_{ji} = \sum_{k=1}^{n} A_{jk}B_{ki} = \sum_{k=1} B_{ik}^{\rm T} A_{kj}^{\rm T} = (B^{\rm T}A^{\rm T})_{ij}
.\end{eqnarray}
Hence,
\begin{eqnarray}
    \label{eq:prob3-result}
    \eqbox{
    (AB)^{\rm T} = B^{\rm T}A^{\rm T}
    }
.\end{eqnarray}



\prob{1.5}{Show that $(AB)^{\dagger} = B^{\dagger}A^{\dagger}$, which is Eq.~(1.29).}

Recall that the hermitian adjoint of a matrix is just $A^{\dagger} = (A^{\rm T})^{*}$, so
\begin{eqnarray}
    \label{eq:adjoint-AB}
    (AB)^{\dagger} = ((AB)^{\rm T})^{*} = (B^{\rm T}A^{\rm T})^{*}
.\end{eqnarray}
Observe that 
\begin{eqnarray}
    \label{eq:complex-conj-product}
    (AB)^{*}_{ij} = \left( \sum_{k=1}^{n} A_{ik}B_{kj} \right)^{*} = \sum_{k=1}^{n} A^{*}_{ik}B^{*}_{kj} = (A^{*}B^{*})_{ij}
,\end{eqnarray}
so \eref{adjoint-AB} becomes
\begin{eqnarray}
    \label{eq:adjoint-BA}
    \eqbox{
        (AB)^{\dagger} = (B^{\rm T}A^{\rm T})^{*} = (B^{\rm T})^{*}(A^{\rm T})^{*} = B^{\dagger}A^{\dagger}
    }
.\end{eqnarray}



\prob{1.7}{Show that the two $4 \times 4$ matrices (1.46) satisfy Grassman's algebra (1.11) for $n=2$.}


\prob{1.12}{Show that the Minkowski product $(x,y) = \va{x} \cdot \va{y} - x^{0}y^{0}$ of two 4-vectors $x$ and $y$ is an inner product obeying the rules (1.78,1.79,1.84).}


\prob{1.18}{Use the Gram-Schmidt method to find orthonormal linear combinations of the three vectors
\begin{eqnarray}
\label{eq:gram-schmidt-vectors}
    \va{s}_{1} = 
    \begin{pmatrix}
    1 \\
    0\\
    0
    \end{pmatrix},
    \quad
    \va{s}_{1} = 
    \begin{pmatrix}
    1 \\
    1\\
    0
    \end{pmatrix},
    \quad
    \va{s}_{3} = 
    \begin{pmatrix}
    1 \\
    1\\
    1
    \end{pmatrix}
.\end{eqnarray}
}


\prob{1.21}{Show that a linear operator $A$ that is represented by a hermitian matrix (1.167) in an orthonormal basis satisfies $(g,Af) = (Ag,f)$.}


\end{document}
